examples/hoare_logic/blocking_semantics3/blocking_semantics3_ImpExpr_eval_msubst_term_1.v
@@ -425,9 +425,8 @@ simpl.
 rewrite H1.
 rewrite H2; auto.
 apply fresh_in_binop with (t:=t) (t':=t') (op := op).
-apply fresh_in_binop with (t:=t) (t':=t') (op := op);
+apply fresh_in_binop with (t:=t) (t':=t') (op := op).
 admit.
-
 Qed.
 
 
